isabelle/Timeout.thy
@@ -1,0 +1,240 @@
+theory Timeout
+imports Semantics PositiveAccounts QuiescentResult
+begin
+
+fun isClosedAndEmpty :: "TransactionOutput \<Rightarrow> bool" where
+"isClosedAndEmpty (TransactionOutput txOut) = (txOutContract txOut = Close
+                                               \<and> accounts (txOutState txOut) = [])" |
+"isClosedAndEmpty _ = False"
+
+lemma max_of_ge : "ia \<le> i \<Longrightarrow> max (i::int) ia = i"
+  by linarith
+
+lemma reduceStepClose_is_Close : "reduceContractStep env sta Close = Reduced re wa nsta ncon \<Longrightarrow> ncon = Close"
+  apply simp
+  apply (cases "refundOne (accounts sta)")
+  apply simp
+  subgoal for a
+    apply (cases "a")
+    subgoal for aa b
+      apply (cases "aa")
+      by simp
+    done
+  done
+
+lemma reductionLoopClose_is_Close : "reductionLoop env sta Close x y = ContractQuiescent re wa nsta ncon \<Longrightarrow> ncon = Close"
+  apply (induction env sta Close x y rule:reductionLoop.induct)
+  subgoal for env state warnings payments
+    apply (simp only:reductionLoop.simps)
+    apply (cases "reduceContractStep env state Close")
+    subgoal for x11 x12 x13 x14
+      apply (simp del:reductionLoop.simps reduceContractStep.simps add:reduceStepClose_is_Close)
+      using reduceStepClose_is_Close by fastforce
+    apply (simp del:reduceContractStep.simps)
+    apply (simp del:reduceContractStep.simps)
+    done
+  done
+
+lemma reduceClose_is_Close : "reduceContractUntilQuiescent env sta Close = ContractQuiescent re wa nsta ncon \<Longrightarrow> ncon = Close"
+  apply (simp del:reductionLoop.simps)
+  using reductionLoopClose_is_Close by blast
+
+lemma timedOutReduce_only_quiescent_in_close_When :
+  "minSlot sta \<le> iniSlot \<Longrightarrow>
+   maxTimeContract (When x41 x42 x43) \<le> iniSlot \<Longrightarrow>
+   iniSlot \<le> endSlot \<Longrightarrow>
+   reduceContractStep \<lparr>slotInterval = (iniSlot, endSlot)\<rparr> (sta\<lparr>minSlot := iniSlot\<rparr>) (When x41 x42 x43) \<noteq> NotReduced"
+  apply (induction x41)
+  by simp_all
+
+lemma maxTimeWhen : "maxTimeContract (When x41 x42 x43) \<le> iniSlot \<Longrightarrow> x42 \<le> iniSlot"
+  apply (induction x41 arbitrary:x42 x43 iniSlot)
+  by auto
+
+lemma maxTimeNotAmbiguous_reduceStep :
+   "maxTimeContract cont \<le> iniSlot \<Longrightarrow>
+    iniSlot \<le> endSlot \<Longrightarrow>
+    reduceContractStep \<lparr>slotInterval = (iniSlot, endSlot)\<rparr> state cont \<noteq> AmbiguousSlotIntervalReductionError"
+  apply (cases cont)
+  apply simp
+  apply (auto split:option.split bool.split)
+  subgoal for x21 x22 x23 x24 x25
+    apply (cases "let moneyToPay = evalValue \<lparr>slotInterval = (iniSlot, endSlot)\<rparr> state x24 in moneyToPay \<le> 0")
+    apply simp
+    apply simp
+    apply (cases "let moneyToPay = evalValue \<lparr>slotInterval = (iniSlot, endSlot)\<rparr> state x24;
+                      balance = case lookup (x21, x23) (accounts state) of None \<Rightarrow> 0 | Some x \<Rightarrow> x; paidMoney = min balance moneyToPay
+                  in giveMoney x22 x23 paidMoney (if balance \<le> moneyToPay then MList.delete (x21, x23) (accounts state)
+                                                  else MList.insert (x21, x23) (balance - paidMoney) (accounts state))")
+    by (metis ReduceStepResult.distinct(3) case_prod_conv)
+  using maxTimeWhen apply blast
+  by (meson ReduceStepResult.distinct(3))
+
+lemma maxTimeOnlyDecreases_reduceStepWhen :
+  "reduceContractStep inte state (When x41 x42 x43) = Reduced wa ef nstate ncont \<Longrightarrow>
+   maxTimeContract ncont \<le> maxTimeContract (When x41 x42 x43)"
+  apply (induction x41 arbitrary: inte state x42 x43 wa ef nstate ncont)
+  apply (smt ReduceStepResult.distinct(1) ReduceStepResult.distinct(3) ReduceStepResult.inject maxTimeContract.simps(4) prod.case_eq_if reduceContractStep.simps(4))
+  by fastforce
+
+lemma maxTimeOnlyDecreases_reduceStep :
+  "reduceContractStep inte state cont = Reduced wa ef nstate ncont \<Longrightarrow>
+   maxTimeContract ncont \<le> maxTimeContract cont"
+  apply (cases cont)
+  using reduceStepClose_is_Close apply blast
+  apply (simp only:reduceContractStep.simps)
+  subgoal for x21 x22 x23 x24 x25
+    apply (cases "let moneyToPay = evalValue inte state x24
+                  in evalValue inte state x24 \<le> 0")
+    apply simp
+    apply simp
+    apply (cases "let moneyToPay = evalValue inte state x24; balance = case lookup (x21, x23) (accounts state) of None \<Rightarrow> 0 | Some x \<Rightarrow> x;
+                      paidMoney = min balance moneyToPay
+                  in giveMoney x22 x23 paidMoney
+                               (if balance \<le> moneyToPay then MList.delete (x21, x23) (accounts state)
+                                else MList.insert (x21, x23) (balance - paidMoney) (accounts state))")
+    by (metis ReduceStepResult.inject case_prod_conv eq_iff)
+    apply auto[1]
+  apply (simp add: maxTimeOnlyDecreases_reduceStepWhen)
+  by (metis ReduceStepResult.inject eq_iff maxTimeContract.simps(6) reduceContractStep.simps(5))
+
+lemma maxTimeNotAmbiguous_reduceLoop : "maxTimeContract cont \<le> iniSlot \<Longrightarrow>
+    iniSlot \<le> endSlot \<Longrightarrow>
+    reductionLoop \<lparr>slotInterval = (iniSlot, endSlot)\<rparr> sta cont x y \<noteq> RRAmbiguousSlotIntervalError"
+  apply (induction "\<lparr>slotInterval = (iniSlot, endSlot)\<rparr>" sta cont x y rule:reductionLoop.induct)
+  subgoal premises facts for state contract warnings payments
+    apply (cases "reduceContractStep \<lparr>slotInterval = (iniSlot, endSlot)\<rparr> state contract")
+      apply (simp only:reductionLoop.simps ReduceStepResult.case)
+      apply (simp only:Let_def)
+      using facts(1) facts(2) facts(3) maxTimeOnlyDecreases_reduceStep apply fastforce
+      apply auto[1]
+      by (simp add: facts(2) facts(3) maxTimeNotAmbiguous_reduceStep)
+    done
+
+lemma maxTimeNotAmbiguous : "maxTimeContract cont \<le> iniSlot \<Longrightarrow>
+       iniSlot \<le> endSlot \<Longrightarrow>
+       reduceContractUntilQuiescent \<lparr>slotInterval = (iniSlot, endSlot)\<rparr> (sta\<lparr>minSlot := iniSlot\<rparr>) cont \<noteq> RRAmbiguousSlotIntervalError"
+  using maxTimeNotAmbiguous_reduceLoop by auto
+
+
+lemma timedOutReduce_only_quiescent_in_close :
+  "minSlot sta \<le> iniSlot \<Longrightarrow>
+   maxTimeContract c \<le> iniSlot \<Longrightarrow>
+   iniSlot \<le> endSlot \<Longrightarrow>
+   reduceContractStep \<lparr>slotInterval = (iniSlot, endSlot)\<rparr> (sta\<lparr>minSlot := iniSlot\<rparr>) c = NotReduced \<Longrightarrow> c = Close"
+  apply (cases c)
+  apply blast
+  apply (metis reduceContractStep.simps(2) reduceContractStepPayIsQuiescent)
+  apply simp
+  using timedOutReduce_only_quiescent_in_close_When apply blast
+  by (metis ReduceStepResult.distinct(1) reduceContractStep.simps(5))
+
+lemma timedOutReduceStep_does_not_modify_minSlot :
+  "minSlot sta = iniSlot \<Longrightarrow>
+   reduceContractStep \<lparr>slotInterval = (iniSlot, endSlot)\<rparr> sta contract =
+   Reduced warning effect newState ncontract \<Longrightarrow> minSlot newState = iniSlot"
+  apply (cases contract)
+    apply simp
+    apply (cases "refundOne (accounts sta)")
+      apply simp
+      subgoal for a
+        apply (cases a)
+        subgoal for aa
+          apply (cases aa)
+          by auto
+        done
+      subgoal for x21 x22 x23 x24
+      apply (cases "let moneyToPay = evalValue \<lparr>slotInterval = (iniSlot, endSlot)\<rparr> sta x24
+                    in moneyToPay \<le> 0")
+      apply auto[1]
+      apply simp
+      apply (cases "giveMoney x22 x23
+           (min (case lookup (x21, x23) (accounts sta) of None \<Rightarrow> 0 | Some x \<Rightarrow> x)
+             (evalValue \<lparr>slotInterval = (iniSlot, endSlot)\<rparr> sta x24))
+           (if (case lookup (x21, x23) (accounts sta) of None \<Rightarrow> 0 | Some x \<Rightarrow> x)
+               \<le> evalValue \<lparr>slotInterval = (iniSlot, endSlot)\<rparr> sta x24
+            then MList.delete (x21, x23) (accounts sta)
+            else MList.insert (x21, x23)
+                  ((case lookup (x21, x23) (accounts sta) of None \<Rightarrow> 0 | Some x \<Rightarrow> x) -
+                   min (case lookup (x21, x23) (accounts sta) of None \<Rightarrow> 0 | Some x \<Rightarrow> x)
+                    (evalValue \<lparr>slotInterval = (iniSlot, endSlot)\<rparr> sta x24))
+                  (accounts sta))")
+      by (auto simp:Let_def)
+      apply auto[1]
+    apply (smt ReduceStepResult.distinct(1) ReduceStepResult.distinct(3) ReduceStepResult.inject State.ext_inject State.surjective State.update_convs(4) prod.case_eq_if reduceContractStep.simps(4))
+    by (smt ReduceStepResult.inject State.ext_inject State.surjective State.update_convs(3) State.update_convs(4) reduceContractStep.simps(5))
+
+lemma timedOutReduceContractLoop_closes_contract : "minSlot sta \<le> iniSlot \<Longrightarrow>
+    maxTimeContract cont \<le> iniSlot \<Longrightarrow>
+    iniSlot \<le> endSlot \<Longrightarrow>
+    minSlot sta = iniSlot \<Longrightarrow>
+    reductionLoop \<lparr>slotInterval = (iniSlot, endSlot)\<rparr> sta cont x y =
+    ContractQuiescent warning effect newState ncontract \<Longrightarrow>
+    ncontract = Close"
+  apply (induction "\<lparr>slotInterval = (iniSlot, endSlot)\<rparr>" sta cont x y arbitrary: warning effect newState ncontract rule:reductionLoop.induct)
+  subgoal for state contract warnings payments warning effect newState ncontract
+    apply (simp only:reductionLoop.simps[of "\<lparr>slotInterval = (iniSlot, endSlot)\<rparr>" "(sta\<lparr>minSlot := iniSlot\<rparr>)" contract warnings payments])
+    apply (cases "reduceContractStep \<lparr>slotInterval = (iniSlot, endSlot)\<rparr> state contract")
+    subgoal for x11 x12 x13 x14
+      apply (simp only:ReduceStepResult.case Let_def)
+      subgoal premises facts
+        apply (rule facts(1)[of x11 x12 x13 x14 "(if x11 = ReduceNoWarning then warnings else x11 # warnings)"
+                                "(case x12 of ReduceNoPayment \<Rightarrow> payments | ReduceWithPayment payment \<Rightarrow> payment # payments)"
+                                warning effect newState ncontract])
+        apply simp
+        apply simp
+        apply simp
+        apply simp
+        using facts(3) facts(7) maxTimeOnlyDecreases_reduceStep apply fastforce
+        apply simp
+        using facts(5) facts(7) timedOutReduceStep_does_not_modify_minSlot apply blast
+        by (metis (no_types, lifting) ReduceStepResult.simps(8) facts(6) facts(7) reductionLoop.simps)
+      done
+    using timedOutReduce_only_quiescent_in_close apply fastforce
+    using maxTimeNotAmbiguous_reduceStep by blast
+  done
+
+lemma timedOutReduceContractUntilQuiescent_closes_contract :
+  "iniSlot \<ge> minSlot sta
+   \<Longrightarrow> iniSlot \<ge> maxTimeContract cont
+   \<Longrightarrow> endSlot \<ge> iniSlot
+   \<Longrightarrow> reduceContractUntilQuiescent \<lparr>slotInterval = (max iniSlot (minSlot sta), endSlot)\<rparr> (sta\<lparr>minSlot := max iniSlot (minSlot sta)\<rparr>) cont
+   = ContractQuiescent warning effect newState ncontract \<Longrightarrow> ncontract = Close"
+  apply (simp only:reduceContractUntilQuiescent.simps)
+  by (smt State.select_convs(4) State.surjective State.update_convs(4) timedOutReduceContractLoop_closes_contract)
+
+lemma timedOutReduceContractStep_empties_accounts :
+  "validAndPositive_state sta \<Longrightarrow>
+    minSlot sta \<le> iniSlot \<Longrightarrow>
+    maxTimeContract cont \<le> iniSlot \<Longrightarrow>
+    iniSlot \<le> endSlot \<Longrightarrow>
+    reduceContractUntilQuiescent \<lparr>slotInterval = (iniSlot, endSlot)\<rparr> (sta\<lparr>minSlot := iniSlot\<rparr>) cont
+     = ContractQuiescent warning effect newState ncontract \<Longrightarrow> accounts newState = []"
+  by (smt State.ext_inject State.surjective State.update_convs(4) allAccountsPositiveState.elims(3) isQuiescent.simps(1) positiveMoneyInAccountOrNoAccountImpliesAllAccountsPositive reduceContractUntilQuiecentIsQuiescent reduceContractUntilQuiescent.simps timedOutReduceContractLoop_closes_contract validAndPositiveImpliesPositive validAndPositiveImpliesValid validAndPositive_state.elims(3) valid_state.simps)
+
+theorem timedOutTransaction_closes_contract :
+  "validAndPositive_state sta
+   \<Longrightarrow> iniSlot \<ge> minSlot sta
+   \<Longrightarrow> iniSlot \<ge> maxTimeContract cont
+   \<Longrightarrow> endSlot \<ge> iniSlot
+   \<Longrightarrow> accounts sta \<noteq> []
+   \<Longrightarrow> isClosedAndEmpty (computeTransaction \<lparr> interval = (iniSlot, endSlot)
+                                            , inputs = [] \<rparr> sta cont)"
+  apply (simp del:validAndPositive_state.simps reduceContractUntilQuiescent.simps add:Let_def)
+  apply (cases "reduceContractUntilQuiescent \<lparr>slotInterval = (max iniSlot (minSlot sta), endSlot)\<rparr> (sta\<lparr>minSlot := max iniSlot (minSlot sta)\<rparr>) cont")
+  apply (simp only:ReduceResult.case list.case ApplyAllResult.case max_of_ge)
+  apply (cases "cont = Close")
+  apply (simp del:validAndPositive_state.simps reduceContractUntilQuiescent.simps)
+  apply (metis maxTimeContract.simps(1) reduceContractUntilQuiescent.simps reductionLoopClose_is_Close timedOutReduceContractStep_empties_accounts)
+  apply (simp del:validAndPositive_state.simps reduceContractUntilQuiescent.simps)
+  apply (metis max.orderE timedOutReduceContractStep_empties_accounts timedOutReduceContractUntilQuiescent_closes_contract)
+  apply (simp del:validAndPositive_state.simps reduceContractUntilQuiescent.simps)
+  using maxTimeNotAmbiguous by auto
+
+theorem timeOutTransaction_closes_contract2 :
+  "validAndPositive_state sta
+   \<Longrightarrow> accounts sta \<noteq> []
+   \<Longrightarrow> \<exists> inp . isClosedAndEmpty (computeTransaction inp sta cont)"
+  by (meson not_less not_less_iff_gr_or_eq timedOutTransaction_closes_contract)
+
+end
